String.of_nat and app lemmas

src/coqutil/Datatypes/String.v
@@ -1,7 +1,7 @@
 Require Import coqutil.Decidable.
 Require Coq.NArith.BinNatDef.
 
-Require Export Coq.Strings.String.
+Require Export Coq.Strings.String. Local Open Scope string_scope.
 
 Module Ascii.
   Definition ltb (c d : Ascii.ascii) : bool := BinNatDef.N.ltb (Ascii.N_of_ascii c) (Ascii.N_of_ascii d).
@@ -63,6 +63,57 @@ Proof. induction k1, k2, k3; strict_order_t. Qed.
 
 Lemma ltb_total : forall k1 k2, ltb k1 k2 = false -> ltb k2 k1 = false -> k1 = k2.
 Proof. induction k1, k2; strict_order_t. Qed.
+
+Require Import Coq.Numbers.DecimalString.
+Require Import Coq.Numbers.DecimalNat.
+
+Definition of_nat(n: nat): string :=
+  DecimalString.NilEmpty.string_of_uint (Nat.to_uint n).
+
+Lemma string_of_uint_inj: forall n m,
+    NilEmpty.string_of_uint n = NilEmpty.string_of_uint m -> n = m.
+Proof.
+  intros. apply (f_equal NilEmpty.uint_of_string) in H.
+  rewrite 2NilEmpty.usu in H. congruence.
+Qed.
+
+Lemma of_nat_inj: forall n m, of_nat n = of_nat m -> n = m.
+Proof.
+  unfold of_nat. intros.
+  apply string_of_uint_inj in H.
+  apply Unsigned.to_uint_inj in H.
+  exact H.
+Qed.
+
+Lemma app_length: forall (s1 s2: string),
+    length (s1 ++ s2) = (length s1 + length s2)%nat.
+Proof.
+  induction s1; intros. 1: reflexivity. simpl. rewrite IHs1. reflexivity.
+Qed.
+
+Lemma app_inv_l: forall s s1 s2, s1 ++ s = s2 ++ s -> s1 = s2.
+Proof.
+  intros. remember (length s1) as l. remember (length s2) as l2.
+  replace l2 with l in Heql2.
+  2: {
+    apply (f_equal length) in H. rewrite ?app_length in *.
+    eapply (proj1 (PeanoNat.Nat.add_cancel_r _ _ _)) in H. congruence.
+  }
+  revert s1 s2 H Heql Heql2. induction l; intros.
+  - destruct s1; destruct s2; try discriminate. reflexivity.
+  - destruct s1; destruct s2; try discriminate.
+    simpl in H. inversion H. subst a0. clear H. f_equal.
+    simpl in *.
+    eapply PeanoNat.Nat.succ_inj in Heql. eapply PeanoNat.Nat.succ_inj in Heql2.
+    eauto.
+Qed.
+
+Lemma app_inv_r: forall s s1 s2, s ++ s1 = s ++ s2 -> s1 = s2.
+Proof.
+  intros. induction s; intros.
+  - assumption.
+  - simpl in H. inversion H. auto.
+Qed.
 
 #[global] Instance eqb_spec: EqDecider eqb.
 Proof.
